Add patterns option for cases builder

Aesop/Builder/Cases.lean
@@ -5,25 +5,70 @@ Authors: Jannis Limperg
 -/
 
 import Aesop.Builder.Basic
+import Aesop.RuleTac.Cases
 
 open Lean
 open Lean.Meta
 
 namespace Aesop
 
-def RuleBuilder.cases (opts : RegularBuilderOptions) : RuleBuilder :=
+namespace CasesPattern
+
+def check (decl : Name) (p : CasesPattern) : MetaM Unit :=
+  withoutModifyingState do
+    let p ← p.toExpr
+    unless p.isAppOf' decl do
+      throwError "expected pattern '{p}' ({toString p}) to be an application of '{decl}'"
+
+def toIndexingMode (p : CasesPattern) : MetaM IndexingMode :=
+  withoutModifyingState do
+    .hyps <$> DiscrTree.mkPathWithTransparency (← p.toExpr) indexingTransparency
+
+end CasesPattern
+
+
+structure CasesBuilderOptions extends RegularBuilderOptions where
+  patterns : Array CasesPattern
+
+namespace CasesBuilderOptions
+
+protected def default : CasesBuilderOptions where
+  toRegularBuilderOptions := .default
+  patterns := #[]
+
+def indexingMode (decl : Name) (opts : CasesBuilderOptions) :
+    MetaM IndexingMode :=
+  opts.getIndexingModeM do
+    if opts.patterns.isEmpty then
+      IndexingMode.hypsMatchingConst decl
+    else
+      .or <$> opts.patterns.mapM (·.toIndexingMode)
+
+def target (decl : Name) (opts : CasesBuilderOptions) : CasesTarget :=
+  if opts.patterns.isEmpty then
+    .decl decl
+  else
+    .patterns opts.patterns
+
+
+end CasesBuilderOptions
+
+
+def RuleBuilder.cases (opts : CasesBuilderOptions) : RuleBuilder :=
   RuleBuilder.ofGlobalRuleBuilder BuilderName.cases λ phase decl => do
     if let (.norm) := phase then throwError
-      "aesop: cases builder cannot currently be used for norm rules."
+      "cases builder cannot currently be used for norm rules."
       -- TODO `Meta.cases` may assign and introduce metavariables.
       -- (Specifically, it can *replace* existing metavariables, which Aesop
       -- counts as an assignment and an introduction.)
     let inductInfo ← RuleBuilder.checkConstIsInductive name decl
+    opts.patterns.forM (·.check decl)
+    let indexingMode ← opts.indexingMode decl
+    let target := opts.target decl
     return RuleBuilderResult.regular {
       builder := name
-      tac := .cases decl (isRecursiveType := inductInfo.isRec)
-      indexingMode := ← opts.getIndexingModeM $
-        IndexingMode.hypsMatchingConst decl
+      tac := .cases target (isRecursiveType := inductInfo.isRec)
+      indexingMode
       mayUseBranchState := false
     }
   where
