Aesop/RuleTac/Cases.lean
@@ -9,54 +9,70 @@ import Aesop.RuleTac.Basic
 open Lean
 open Lean.Meta
 
-namespace Aesop.RuleTac
+namespace Aesop
 
-partial def cases (decl : Name) (isRecursiveType : Bool) : RuleTac :=
+namespace CasesPattern
+
+-- NOTE: introduces fresh metavariables for the 'holes' in `p`.
+def toExpr (p : CasesPattern) : MetaM Expr := do
+  let (_, _, p) ← openAbstractMVarsResult p
+  return p
+
+end CasesPattern
+
+
+namespace RuleTac
+
+partial def cases (target : CasesTarget) (isRecursiveType : Bool) : RuleTac :=
   SimpleRuleTac.toRuleTac λ input => do
     let goals? ← go #[] #[] input.goal
     match goals? with
-    | none => throwError "No hypothesis of type {decl} found"
+    | none => throwError "No matching hypothesis found."
     | some goals => return goals.toList
   where
     findFirstApplicableHyp (excluded : Array FVarId) (goal : MVarId) :
         MetaM (Option FVarId) :=
       withMVarContext goal do
-        return (← getLCtx).findDecl? λ ldecl =>
-          if ! ldecl.isAuxDecl &&
-             ldecl.type.isAppOf decl &&
-             ! excluded.contains ldecl.fvarId then
-          -- Note: We currently check for occurrences of `decl` structurally,
-          -- not up to WHNF.
-            some ldecl.fvarId
+        let «match» ldecl : MetaM Bool :=
+          match target with
+          | .decl d => withoutModifyingState do
+            return (← matchAppOf (← mkConstWithFreshMVarLevels d) ldecl.type).isSome
+          | .patterns ps => ps.anyM λ p => withoutModifyingState do
+              isDefEq (← p.toExpr) ldecl.type
+              -- TODO `p.toExpr` is mildly expensive, so it would be nicer if
+              -- we didn't have to do this all the time. But we must be careful
+              -- not to leak metavariables.
+        return ← (← getLCtx).findDeclM? λ ldecl => do
+          if ← (pure $ ! ldecl.isAuxDecl) <&&>
+             «match» ldecl <&&>
+             pure (! excluded.contains ldecl.fvarId) then
+            return some ldecl.fvarId
           else
-            none
+            return none
 
     go (newGoals : Array MVarId) (excluded : Array FVarId)
         (goal : MVarId) : MetaM (Option (Array MVarId)) := do
       let (some hyp) ← findFirstApplicableHyp excluded goal
         | return none
-      try
-        let goals ← Meta.cases goal hyp
-        let mut newGoals := newGoals
-        for g in goals do
-          let excluded :=
-            if ! isRecursiveType then
-              excluded
-            else
-              let excluded := excluded.map λ fvarId =>
-                match g.subst.find? fvarId with
-                | some (Expr.fvar fvarId' ..) => fvarId'
-                | _ => fvarId
-              let fields := g.fields.filterMap λ
-                | (Expr.fvar fvarId' ..) => some fvarId'
-                | _ => none
-              excluded ++ fields
-          let newGoals? ← go newGoals excluded g.mvarId
-          match newGoals? with
-          | some newGoals' => newGoals := newGoals'
-          | none => newGoals := newGoals.push g.mvarId
-        return some newGoals
-      catch e =>
-        return none
+      let goals ← try Meta.cases goal hyp catch _ => return none
+      let mut newGoals := newGoals
+      for g in goals do
+        let excluded :=
+          if ! isRecursiveType then
+            excluded
+          else
+            let excluded := excluded.map λ fvarId =>
+              match g.subst.find? fvarId with
+              | some (.fvar fvarId' ..) => fvarId'
+              | _ => fvarId
+            let fields := g.fields.filterMap λ
+              | (.fvar fvarId' ..) => some fvarId'
+              | _ => none
+            excluded ++ fields
+        let newGoals? ← go newGoals excluded g.mvarId
+        match newGoals? with
+        | some newGoals' => newGoals := newGoals'
+        | none => newGoals := newGoals.push g.mvarId
+      return some newGoals
 
 end Aesop.RuleTac
