tests/Cases.lean
@@ -9,10 +9,23 @@ set_option aesop.check.all true
 
 @[aesop 50% cases]
 inductive FancyAnd (α β : Prop) : Prop
-| dummy (p : Empty)
-| and (a : α) (b : β)
+  | dummy (p : Empty)
+  | and (a : α) (b : β)
 
 attribute [aesop safe -51 cases] Empty
 
 example {α β} (h : FancyAnd α β) : α ∧ β := by
+  aesop
+
+@[aesop safe (cases (patterns := [All _ [], All _ (_ :: _)]))]
+inductive All (P : α → Prop) : List α → Prop
+  | nil : All P []
+  | cons : P x → All P xs → All P (x :: xs)
+
+@[aesop 99% constructors]
+structure MyTrue : Prop
+
+-- Without the patterns on the `cases` rule for `All`, this test would loop
+-- since the `constructors` rule would never be applied.
+example {P : α → Prop} (h : All P (x :: xs)) : MyTrue := by
   aesop
